\documentclass[12pt]{letter}
\usepackage{amsmath}
\usepackage{amsfonts}
\usepackage{amssymb}

\begin{document}
	\begin{center}
		\begin{large} Homework 1 Answers \end{large}
	\end{center}

	\begin{enumerate}

		\item
		
		\item Beta-reduce lambda expression:
		\begin{itemize}
			\item[] $(((\lambda x.\lambda y.\lambda z.((x~y)~z)~\lambda f.\lambda a.(f~a))~\lambda i.i)~\lambda j.j)$
			\item[$\rightarrow$]
			$((\lambda y.\lambda z.((\lambda f.\lambda a.(f~a)~y)~z)~\lambda i.i)~\lambda j.j)$
			\item[$\rightarrow$]
			$(\lambda z.((\lambda f.\lambda a.(f~a)~\lambda i.i)~z)~\lambda j.j)$
			\item[$\rightarrow$]
			$((\lambda f.\lambda a.(f~a)~\lambda i.i)~\lambda j.j)$
			\item[$\rightarrow$]
			$(\lambda a.(\lambda i.i~a)~\lambda j.j)$
			\item[$\rightarrow$]
			$(\lambda i.i~\lambda j.j)$
			\item[$\rightarrow$]
			$\lambda j.j$
		\end{itemize}
		
		\item Beta-reduce lambda expression:
		\begin{itemize}
			\item[]
			$(\lambda h.((\lambda a.\lambda f.(f~a)~h)~h)~\lambda f.(f~f))$
			\item[$\rightarrow$]
			$(\lambda h.(\lambda f.(f~h)~h)~\lambda f.(f~f))$
			\item[$\rightarrow$]
			$(\lambda h.(h~h)~\lambda f.(f~f))$
			\item[$\rightarrow$]
			$(\lambda f.(f~f)~\lambda f.(f~f))$
			\item[$\rightarrow$]
			$(\lambda f.(f~f)~\lambda f.(f~f))$
			... and repeat to infinity and beyond.
		\end{itemize}
		
		\item Use $\alpha$ conversion to ensure unique names in the following expression:
		\begin{itemize}
			\item[]
			$\lambda x.\lambda y.(\lambda x.y~\lambda y.x)$
			\item[$\rightarrow$]
			$\lambda x.\lambda y.(\lambda m.y~\lambda n.x)$
		\end{itemize}
		
		\item Define a λ calculus representation for implies. You
should be able to reduce your answer down so that it's in terms
of x, and y and maybe true, and/or false. Notice, when X is true,
Implies is the same as Y and when X is False, Implies is True.
			Assuming:
			\begin{itemize}
				\item $def cond = λe1.λe2.λc.((c~e1)~e2)$
				\item $def not = λx.(((cond~false)~true)~x)$
				\item $def or= λx.λy.((x~true)~y)$
			\end{itemize}

			We have:
			\begin{itemize}
				\item[]
				$(or~(not~x)~y)$
				\item[$\rightarrow$]
				$((\lambda x.\lambda y.((x~true)~y) (\lambda x.(((cond~false)~true)~x)~x))~y)$
				\item[$\rightarrow$]
				$(\lambda y.(((\lambda x.(((cond~false)~true)~x)~x)~true)~y)~y)$
				\item[$\rightarrow$]
				$(((\lambda x.(((cond~false)~true)~x)~x)~true)~y)$
				\item[$\rightarrow$]
				$(((((cond~false)~true)~x)~true)~y)$
				\item[$\rightarrow$]
				$((((\lambda e2.\lambda c.((c~false)~e2)~true)~x)~true)~y)$
				\item[$\rightarrow$]
				$(((\lambda c.((c~false)~true)~x)~true)~y)$
				\item[$\rightarrow$]
				$((((x~false)~true)~true)~y)$
			\end{itemize}
			
			Interpretation: If $x$ is false then the expression is $true$, otherwise the expression is equal to $y$.
			
	\end{enumerate}

\end{document}
